# Please find the values of the following Y-combinators upon reduction:

Make the assumptions that `Y` and `T` stand for the following functions:

```
Y = λt.(λx. t(x x))(λx.t (x x))

T = λf. λn. if (= n 1) 1
                (* n (f (- n 1)))
```

## (**Y** _<u>T</u>_ ) 2

This is an extended version of the above expression:

```
( λt.(λx. t(x x))(λx.t (x x)) T) 2
```

Understanding that Y is a feedback loop, and T is a basic factorial block, we can see that the output of `T 2` will be multiplied to `T 1`.

When applying `2` to `T`, we must first substitute `T` into `f` and `2` into `n`:

```
if (= 2 1) 1
    (* 2 (T (- 2 1)))
```

Note that the predicate if-expression will evaluate to false because 2 != 1, and the expression `(* 2 (T (- 2 1)))` will be evaluated instead. This further simplifies to `(* 2 (T 1))`.

Using the same logic as when applying `2` to `T`, we shall do the same with `1`:

```
if (= 1 1) 1
    (* 1 (T (- 1 1)))
```

In this iteration of `T`, the predicate if-expression will evaluate to true, which will return a result of `1`.

Let's take an inventory of what we have so far:

```
( λt.(λx. t(x x))(λx.t (x x)) T) 2 => Master formula

(* 2 (T 1)) => Output of (T 2)

1 => Output of (T 1)
```

When multiplying the results, we shall get 2 in the output.

**Final Answer: 2**

## (**Y** _<u>T</u>_ ) 1

Understanding that Y is a feedback loop, and T is a basic factorial block, we can see that the output of `T 1` will be where the buck stops.

When applying `1` to `T`, we must first substitute `T` into `f` and `1` into `n`:

```
if (= 1 1) 1
    (* 1 (T (- 1 1)))
```

In this iteration of `T`, the predicate if-expression will evaluate to true, which will return a result of `1`.

**Final Answer: 1**
