# Reduce the following lambda expression:

```
(λx . λy . (add y ((λz . (mul x z)) 3))) 7 5
```

The first order of operation is to apply beta reduction and apply `7` to `x` such that:
`(λy . (add y ((λz . (mul 7 z)) 3))) 5`

Then we apply `5` to `y` such that:
`add 5 ((λz . (mul 7 z)) 3)`

We note that in the above equation, the subexpression `(λz . (mul 7 z)) 3` can simplify to `(mul 7 3)`.

As a result, we have the expression `add 5 (mul 7 3)`, which then simplifies to `26`.

**Final Answer: 26**